theories/lang/cpp/logic/layout.v
@@ -29,14 +29,14 @@ Section with_Σ.
   Axiom union_padding_timeless : forall q cls idx, Timeless (union_padding resolve q cls idx).
   Axiom union_padding_frac_valid : forall (q : Qp) cls idx, Observe [| q ≤ 1 |]%Qp (union_padding resolve q cls idx).
 
-  Global Existing Instances
+  #[global] Existing Instances
     struct_padding_fractional struct_padding_timeless struct_padding_frac_valid
     union_padding_fractional union_padding_timeless union_padding_frac_valid.
 
-  Global Instance struct_padding_as_fractional q cls :
+  #[global] Instance struct_padding_as_fractional q cls :
     AsFractional (struct_padding resolve q cls) (λ q, struct_padding resolve q cls) q.
   Proof. exact: Build_AsFractional. Qed.
-  Global Instance union_padding_as_fractional q cls idx :
+  #[global] Instance union_padding_as_fractional q cls idx :
     AsFractional (union_padding resolve q cls idx) (λ q, union_padding resolve q cls idx) q.
   Proof. exact: Build_AsFractional. Qed.
 
@@ -65,22 +65,113 @@ Section with_Σ.
   Axiom raw_bytes_of_sizeof : forall ty v rs,
      raw_bytes_of_val resolve ty v rs -> size_of resolve ty = Some (N.of_nat $ length rs).
 
-  (* TODO confirm that this is correct with respect to our model. *)
-  Definition rawR (rs : list raw_byte) (q : Qp) : Rep :=
-    arrayR T_uchar (fun r => primR T_uchar q (Vraw r)) rs.
+  (** [rawR q rs]: the argument pointer points to [raw_byte] [r] within the C++ abstract machine. *)
+  Definition rawR_def (q : Qp) (r : raw_byte) : Rep :=
+    as_Rep (fun p => tptsto T_uchar q p (Vraw r)).
+  Definition rawR_aux : seal (@rawR_def). Proof. by eexists. Qed.
+  Definition rawR := rawR_aux.(unseal).
+  Definition rawR_eq : @rawR = _ := rawR_aux.(seal_eq).
+  #[global] Arguments rawR q raw : rename.
 
-  Axiom primR_to_rawR: forall ty q v,
-    primR ty q v -|- Exists rs, rawR rs q ** [| raw_bytes_of_val resolve ty v rs |] ** type_ptrR ty.
+  #[global] Instance rawR_proper :
+    Proper ((=) ==> (=) ==> (⊣⊢)) (@rawR).
+  Proof. by intros ??-> ??->. Qed.
+  #[global] Instance rawR_mono :
+    Proper ((=) ==> (=) ==> (⊢)) (@rawR).
+  Proof. by intros ??-> ??->. Qed.
+
+  #[global] Instance rawR_affine q raw
+    : Affine (rawR q raw).
+  Proof. rewrite rawR_eq. apply _. Qed.
+  #[global] Instance rawR_timeless q raw
+    : Timeless (rawR q raw).
+  Proof. rewrite rawR_eq. apply _. Qed.
+
+  #[global] Instance rawR_fractional raw :
+    Fractional (λ q, rawR q raw).
+  Proof. rewrite rawR_eq. apply _. Qed.
+  #[global] Instance rawR_as_fractional q raw :
+    AsFractional (rawR q raw) (λ q, rawR q raw) q.
+  Proof. constructor. done. apply _. Qed.
+
+  #[global] Instance rawR_observe_frac_valid (q : Qp) raw :
+    Observe [| q ≤ 1 |]%Qp (rawR q raw).
+  Proof. rewrite rawR_eq. apply _. Qed.
+
+  #[global] Instance rawR_observe_agree q1 q2 raw1 raw2 :
+    Observe2 [| raw1 = raw2 |] (rawR q1 raw1) (rawR q2 raw2).
+  Proof.
+    rewrite rawR_eq/rawR_def.
+    apply: as_Rep_only_provable_observe_2=> p.
+    iIntros "Hptsto1 Hptsto2".
+    iPoseProof (tptsto_agree_raw with "Hptsto1 Hptsto2") as "%Hraws"; eauto.
+    iModIntro; iPureIntro; by inversion Hraws.
+  Qed.
+
+  Definition rawsR (q : Qp) (rs : list raw_byte) : Rep := arrayR T_uchar (rawR q) rs.
+
+  #[global] Instance rawsR_proper :
+    Proper ((=) ==> (=) ==> (⊣⊢)) (@rawsR).
+  Proof. by intros ??-> ??->. Qed.
+  #[global] Instance rawsR_mono :
+    Proper ((=) ==> (=) ==> (⊢)) (@rawsR).
+  Proof. by intros ??-> ??->. Qed.
+
+  #[global] Instance rawsR_affine q rs
+    : Affine (rawsR q rs).
+  Proof. apply _. Qed.
+  #[global] Instance rawsR_timeless q rs
+    : Timeless (rawsR q rs).
+  Proof. apply _. Qed.
+
+  #[global] Instance rawsR_fractional rs :
+    Fractional (λ q, rawsR q rs).
+  Proof. apply _. Qed.
+  #[global] Instance rawsR_as_fractional q rs :
+    AsFractional (rawsR q rs) (λ q, rawsR q rs) q.
+  Proof. constructor. done. apply _. Qed.
+
+  #[global] Instance rawsR_observe_frac_valid (q : Qp) rs :
+    (0 < length rs) ->
+    Observe [| q ≤ 1 |]%Qp (rawsR q rs).
+  Proof.
+    intros Hlen; rewrite /rawsR; induction rs;
+      by [ simpl in Hlen; lia
+         | rewrite arrayR_cons; apply _].
+  Qed.
+
+  #[global] Instance rawsR_observe_agree q1 q2 rs1 rs2 :
+    length rs1 = length rs2 ->
+    Observe2 [| rs1 = rs2 |] (rawsR q1 rs1) (rawsR q2 rs2).
+  Proof.
+    generalize dependent rs2; induction rs1 as [| r1 ? ?]; intros * Hlen.
+    - destruct rs2; [| simpl in Hlen; lia].
+      rewrite /Observe2; iIntros "? ? !>"; by iPureIntro.
+    - destruct rs2 as [| r2 ?]; [simpl in Hlen; lia |].
+      rewrite !cons_length in Hlen; inversion Hlen.
+      rewrite /rawsR !arrayR_cons;
+        fold (rawsR q1 rs1);
+        fold (rawsR q2 rs2).
+      iIntros "(Htype_ptrR1 & HrawR1 & HrawsR1)
+               (Htype_ptrR2 & HrawR2 & HrawsR2)".
+      iDestruct (observe_2 [| r1 = r2 |] with "HrawR1 HrawR2") as %->.
+      specialize (IHrs1 rs2 ltac:(auto)).
+      iDestruct (observe_2 [| rs1 = rs2 |] with "HrawsR1 HrawsR2") as %->.
+      iModIntro; by iPureIntro.
+  Qed.
+
+  Axiom primR_to_rawsR: forall ty q v,
+    primR ty q v -|- Exists rs, rawsR q rs ** [| raw_bytes_of_val resolve ty v rs |] ** type_ptrR ty.
 
   (* TODO: Do we need type_ptrR here? *)
   Axiom struct_to_raw : forall cls st rss q,
     glob_def resolve cls = Some (Gstruct st) ->
     st.(s_layout) = POD ->
     ([∗ list] fld ∈ st.(s_fields), let '(n,ty,_,_) := fld in
-       Exists r, [| rss !! n = Some r |] **
-       _offsetR (_field {| f_name := n ; f_type := cls |}) (rawR r q))
+       Exists rs, [| rss !! n = Some rs |] **
+       _offsetR (_field {| f_name := n ; f_type := cls |}) (rawsR q rs))
       ** struct_padding resolve q cls -|-
-      Exists rs, rawR rs q ** [| raw_bytes_of_struct resolve cls rss rs |].
+      Exists rs, rawsR q rs ** [| raw_bytes_of_struct resolve cls rss rs |].
 
   (** decompose a struct into its constituent fields and base classes.
    *)
@@ -134,8 +225,7 @@ Section with_Σ.
       raw_bytes_of_val resolve (Tint sz Unsigned) (Vint x) rs <-> (exists l, decodes_uint l x /\ rs = raw_int_byte <$> l).
 
   Axiom raw_int_byte_primR : forall q r,
-      primR T_uchar q (Vraw (raw_int_byte r)) -|- primR T_uchar q (Vint (Z.of_N r)).
-
+      rawR q (raw_int_byte r) -|- primR T_uchar q (Vint (Z.of_N r)).
 
   (** TODO: determine whether this is correct with respect to pointers *)
   Lemma decode_uint_primR : forall q sz (x : Z),
@@ -146,18 +236,21 @@ Section with_Σ.
       [| decodes_uint l x |].
   Proof.
     move => q sz x.
-    rewrite primR_to_rawR. setoid_rewrite raw_byte_of_int_eq.
+    rewrite primR_to_rawsR. setoid_rewrite raw_byte_of_int_eq.
     iSplit.
-    - iDestruct 1 as (rs) "(Hraw&H&$)". iDestruct "H" as %[l [Hdec ->]]. iExists _. iSplit => //. clear Hdec.
-      rewrite /rawR arrayR_eq/arrayR_def. iStopProof.
+    - iDestruct 1 as (rs) "(Hraw & H & $)".
+      iDestruct "H" as %[l [Hdec ->]].
+      iExists _; iSplit => //. clear Hdec.
+      rewrite /rawsR arrayR_eq/arrayR_def. iStopProof.
       (* TODO i need to do induction here because the [Proper] instances are too weak. *)
       induction l => // /=.
       rewrite !arrR_cons; eauto.
       rewrite -IHl /=. f_equiv. f_equiv.
         by rewrite raw_int_byte_primR.
-    - iDestruct 1 as (l) "(Harray&$&H)". iDestruct "H" as %Hdec.
-      iExists _. iSplit => //; eauto with iFrame. clear Hdec.
-      rewrite /rawR arrayR_eq/arrayR_def; iStopProof.
+    - iDestruct 1 as (l) "(Harray & $ & H)".
+      iDestruct "H" as %Hdec.
+      iExists _; iSplit => //; eauto with iFrame. clear Hdec.
+      rewrite /rawsR arrayR_eq/arrayR_def; iStopProof.
       induction l => // /=.
       rewrite !arrR_cons; eauto.
       rewrite -IHl /=. f_equiv. f_equiv.
